proved array map2

resources/array_map2/array_map2_old.ml
@@ -1,0 +1,14 @@
+open Combinators
+
+let array_map2 (f: 'a -> 'b -> 'c) (xs: 'a array) (ys: 'b array) =
+  let (len: int) = Array.length xs in
+  if len = 0
+  then [| |]
+  else
+    let (zs: 'c array) = 
+      Array.make len
+        (f xs.(0) ys.(0)) in
+    let _ = for_upto 0 len (fun i -> 
+      zs.(i) <- f xs.(i) ys.(i);
+    ) in
+    zs
