resources/array_map2/Verify_array_map2_old.v
@@ -1,0 +1,72 @@
+Set Implicit Arguments.
+From CFML Require Import WPLib Stdlib.
+From TLC Require Import LibListZ.
+
+From Common Require Import Verify_combinators.
+
+From Common Require Import Tactics Utils Solver.
+
+From ProofsArrayMap2 Require Import Array_map2_old_ml.
+
+Lemma array_map2_spec :
+  forall (A : Type) `{EA : Enc A}  (B : Type) `{EB : Enc B}
+         (C : Type) `{EC : Enc C}
+         (f: func) (xs: array A) (ys: array B)
+         (lx: list A) (ly: list B)
+         (fp: A -> B -> C),
+    (forall (a: A) (b: B),
+        SPEC_PURE (f a b)
+          POST (fun (c: C) => \[c = fp a b])) ->
+    (length lx = length ly) ->
+  SPEC (array_map2 f xs ys)
+  PRE (xs ~> Array lx \* ys ~> Array ly)
+  POST (fun (cs : array C) => xs ~> Array lx \* ys ~> Array ly \*
+                                cs ~> Array (map2 fp (combine lx ly))).
+Proof using (All).
+  xcf.
+  xapp.
+  xif as cond.
+  - xvalemptyarr. { repeat sis_list_solver. }
+  - xinhab.
+    xapp. { sis_handle_int_index_prove. }
+    xinhab_inner A.
+    xapp.  { sis_handle_int_index_prove. }
+    xapp.
+    xalloc cs data Hdata.
+    xletopaque tmp Htmp.
+    xapp (for_upto_spec 0 (length lx) tmp
+            (fun (i: int) =>
+               xs ~> Array lx \*
+               ys ~> Array ly \*
+               cs ~> Array (
+                 take i (map2 fp (combine lx ly))
+                ++ drop i (make (length lx) (fp lx[0] ly[0]))
+               )
+            )
+         ). {
+      sis_solve_start.
+      sis_handle_int_index_prove.
+      unfold map2.
+      rewrite length_take_nonneg; rew_list;
+      try (rewrite length_map, length_eq, length_combine, <- length_eq; math).
+      rewrite length_drop_nonneg; rew_list; try (rewrite length_make; math).
+      sis_handle_take_splitting_goals;
+      try (rewrite length_take_nonneg; auto; unfold map2;
+           rewrite length_map, length_eq, length_combine, <- length_eq; math).
+      rewrite (@take_pos_last _ (Inhab_of_val (fp lx[0] ly[0]))
+                 (map2 fp (combine lx ly)) (i + 1));
+      try (sis_handle_int_index_prove;
+        unfold map2; rewrite length_map, length_eq, length_combine, <- length_eq; math).
+      math_rewrite (i + 1 - 1 = i); rew_list.
+      f_equal.
+      rewrite (@read_map2_combine _ IA0 _ IA); auto.
+      rewrite drop_make_eq; try math.
+      rewrite drop_make_eq; try math.
+      math_rewrite (length lx - i = length lx - (i + 1) + 1).
+      rewrite make_succ_l; try math.
+      rewrite update_zero; auto.
+    }
+    { math. } { rewrite take_zero; simpl; auto. }
+  xmatch.
+  xvals*. { repeat sis_handle_take_drop_full_length; rew_list; auto. }
+Qed.
