resources/common/Verify_arr.v
@@ -3,8 +3,7 @@ Set Implicit Arguments.
 From CFML Require Import WPLib Stdlib.
 From TLC Require Import LibListZ.
 
-From Common Require Import Arr_ml.
-
+From Common Require Import Utils Arr_ml.
 
 Lemma array_iter_spec :
   forall A `{EA: Enc A} (f: func) (a: array A) (l: list A),
@@ -251,3 +250,50 @@ Proof using.
   xapp; rew_list; auto; xsimpl*.
 Qed.
 Arguments array_iteri_spec {A} {EA} f a l I HI.
+
+
+Lemma array_to_list_spec :
+  forall A `{EA: Enc A} (a: array A) (l: list A),
+  SPEC (Array_ml.to_list a)
+    PRE (a ~> Array l)
+    POST (fun (ls: list A) => \[ls = l] \* a ~> Array l).
+Proof using.
+  xcf.
+  xlet as;=> tmp Htmp.
+  assert (forall (i: int) (acc: list A),
+             -1 <= i < length l ->
+             (acc = drop (i + 1) l) ->
+             SPEC (tmp i acc)
+             PRE (a ~> Array l)
+             POST (fun (res: list A) => \[res = l] \* a ~> Array l)
+         ). {
+    intros i; induction_wf IH: (downto (-1)) i. 
+    intros acc Hi Hacc; apply Htmp; clear Htmp.
+    xif;=> cond.
+    - xvals. { rewrite drop_neg in Hacc; subst; try math; auto.  }
+    - assert (IA: Inhab A). {
+        apply Inhab_of_val; destruct l as [| l ls]; rew_list in *; try math; auto.
+      }
+      xapp. { apply int_index_prove; math. }
+      xapp (IH (i - 1)).
+      + apply downto_intro; math.
+      + math.
+      + rewrite Hacc.
+        math_rewrite (i - 1 + 1 = i).
+        rewrite (@list_split_ith _ IA l i) at 3; try math.
+        rewrite drop_app_l; rew_list; try (rewrite length_take_nonneg; math).
+        rewrite drop_app_l; rew_list; try (rewrite length_take_nonneg; math).
+        assert (Hil: i = length (take i l)) by (rewrite length_take_nonneg; math).
+        rewrite Hil at 3; rewrite drop_at_length; rew_list; auto.
+      + xsimpl*.
+  }
+  xapp.
+  xapp. {
+    math.
+  } {
+    math_rewrite (length l - 1 + 1 = length l); rewrite drop_at_length; auto.
+  } {
+    xsimpl*.
+  }
+Qed.  
+Arguments array_to_list_spec {A} {EA} a l.
